Aesop/Script/Check.lean
@@ -1,0 +1,44 @@
+/-
+Copyright (c) 2024 Jannis Limperg. All rights reserved.
+Released under Apache 2.0 license as described in the file LICENSE.
+Authors: Jannis Limperg
+-/
+
+import Aesop.Check
+import Aesop.Script.UScript
+
+open Lean Lean.Elab.Tactic
+open Lean.Parser.Tactic (tacticSeq)
+
+namespace Aesop.Script
+
+def UScript.checkIfEnabled (uscript : UScript) : MetaM Unit := do
+  unless ← Check.script.steps.isEnabled do
+    return
+  try
+    uscript.validate
+  catch e =>
+    throwError "{Check.script.steps.name}: {e.toMessageData}"
+
+end Script
+
+def checkRenderedScriptIfEnabled (script : TSyntax ``tacticSeq)
+    (preState : Meta.SavedState) (goal : MVarId) (expectCompleteProof : Bool) :
+    MetaM Unit := do
+  if ! (← Check.script.isEnabled) then
+    return
+  let go : TacticM Unit := do
+    setGoals [goal]
+    evalTactic script
+    if expectCompleteProof && ! (← getUnsolvedGoals).isEmpty then
+      throwError "script executed successfully but did not solve the main goal"
+  try
+    show MetaM Unit from withoutModifyingState do
+      preState.restore
+      go.run { elaborator := .anonymous, recover := false }
+        |>.run' { goals := [goal] }
+        |>.run'
+  catch e => throwError
+    "{Check.script.name}: error while executing generated script:{indentD e.toMessageData}"
+
+end Aesop
