Aesop/Script/Main.lean
@@ -1,0 +1,55 @@
+/-
+Copyright (c) 2024 Jannis Limperg. All rights reserved.
+Released under Apache 2.0 license as described in the file LICENSE.
+Authors: Jannis Limperg
+-/
+
+import Aesop.Options
+import Aesop.Script.Check
+import Aesop.Script.StructureDynamic
+import Aesop.Script.StructureStatic
+import Aesop.Script.OptimizeSyntax
+
+open Lean
+open Lean.Parser.Tactic (tacticSeq)
+
+namespace Aesop.Script
+
+def UScript.optimize (uscript : UScript)  (preState : Meta.SavedState)
+    (goal : MVarId) : MetaM (Option (TSyntax ``tacticSeq × Bool)) := do
+  let structureResult? ←
+    if aesop.dev.dynamicStructuring.get (← getOptions) then
+      uscript.toSScriptDynamic preState goal
+    else
+      let tacticState ← preState.runMetaM' $ TacticState.mkInitial goal
+      uscript.toSScriptStatic tacticState
+  let some (sscript, perfect) := structureResult?
+    | return none
+  let tacticSeq ← `(tacticSeq| $(← sscript.render):tactic*)
+  let tacticSeq ← optimizeSyntax tacticSeq
+  return (tacticSeq, perfect)
+
+end Script
+
+open Script
+
+def checkAndTraceScript (uscript : UScript)
+    (sscript? : Option (TSyntax ``tacticSeq)) (preState : Meta.SavedState)
+    (goal : MVarId) (options : Aesop.Options') (expectCompleteProof : Bool)
+    (tacticName : String) :
+    MetaM Unit := do
+  if let some script := sscript? then
+    if options.traceScript then
+      addTryThisTacticSeqSuggestion (← getRef) script
+    checkRenderedScriptIfEnabled script preState goal
+      (expectCompleteProof := expectCompleteProof)
+  else
+    if options.traceScript then
+      let tacticSeq ← uscript.renderTacticSeq preState goal
+      addTryThisTacticSeqSuggestion (← getRef) tacticSeq
+    if ← Check.script.isEnabled then
+      throwError "{Check.script.name}: structuring the script failed"
+    else
+      logWarning m!"{tacticName}: structuring the script failed. Reporting unstructured script."
+
+end Aesop
